\batchmode
\documentclass{article}
\usepackage{epsfig}
\pagestyle{empty}
\begin{document}
$\Sigma$
\pagebreak

$>0$
\pagebreak

$P(Y|X)$
\pagebreak

$X$
\pagebreak

$P(Y)$
\pagebreak

$\sum_{n=1}^N {1\over n^s}$
\pagebreak

$\alpha$
\pagebreak

$\beta$
\pagebreak

$ 2\times 3$
\pagebreak

$N \times 2$
\pagebreak

$n$
\pagebreak

$\sqrt(N)$
\pagebreak

$o_i$
\pagebreak

$i$
\pagebreak

$e_i$
\pagebreak

$\Sum_i^N (o_i-e_i)^2/e_i \sim \Chi^2_{N-1}$
\pagebreak

$\chi^2$
\pagebreak

$p$
\pagebreak

$\sqrt{N}$
\pagebreak

$\geq 1$
\pagebreak

$v_i$
\pagebreak

$_{10}(v_i)$
\pagebreak

$(v_i)$
\pagebreak

$-\max < x < \max$
\pagebreak

$ d1 \cdot d2$
\pagebreak

$3 \times 5$
\pagebreak

$(3 \times 5) \cdot (5 \times 3) \rightarrow (3 \times 3)$
\pagebreak

$3 \times 3$
\pagebreak

$5 \times 5$
\pagebreak

$\cdot$
\pagebreak

$(3\times 1)$
\pagebreak

$(3\times 4)$
\pagebreak

$(1 \times 4)$
\pagebreak

$N \times 1$
\pagebreak

$1 \times N$
\pagebreak

$N \times N$
\pagebreak

$v < m1x1+ m2x2 + ... + mnxn$
\pagebreak

$3 < 2x + 4y - 7z$
\pagebreak

$y$
\pagebreak

$0 < y$
\pagebreak

$(-1, +1)$
\pagebreak

$\to$
\pagebreak

$n>1$
\pagebreak

$n\to\infty$
\pagebreak

$\leq$
\pagebreak

$t$
\pagebreak

$\hat{p}$
\pagebreak

$g_1(A) + g_2(BC) + g_3(CD)$
\pagebreak

$R^2$
\pagebreak

$Y$
\pagebreak

$\epsilon$
\pagebreak

$k$
\pagebreak

$ SST \equiv \sum (Y_i - \bar Y) ^2 $
\pagebreak

$ SSE \equiv \sum \epsilon ^2 $
\pagebreak

$ R^2 \equiv 1 - {SSE\over SST} $
\pagebreak

$ R^2_{adj} \equiv R^2 - {(k-1)\over (n-k-1)}(1-R^2) $
\pagebreak

$5 \times 1$
\pagebreak

${\cal N}(0,1)$
\pagebreak

$3 \sigma^4$
\pagebreak

$(\sum_i (x_i - \mu)^3/n))$
\pagebreak

$^{3/2}$
\pagebreak

$n-1$
\pagebreak

$\sum_i (x_i - \mu)^4/n)$
\pagebreak

$ {\hbox{cov}(a,b)\over \sqrt{\hbox{var}(a)} \sqrt{\hbox{var}(b)}}.$
\pagebreak

$\sqrt{\sum_i{(a_i - b_i)^2}},$
\pagebreak

$\sum_i{|a_i - b_i|},$
\pagebreak

$a = b$
\pagebreak

$|a_i - b_i|$
\pagebreak

$L_p$
\pagebreak

$\left(\sum_i{|a_i - b_i|^2}\right)^{1/p}$
\pagebreak

$(X-\mu) / \sigma$
\pagebreak

$\sigma$
\pagebreak

$(X-\mu)$
\pagebreak

$\mu=0, \sigma^2=NaN$
\pagebreak

$N$
\pagebreak

$N/(N-1)$
\pagebreak

$\bar x$
\pagebreak

$\mu$
\pagebreak

$(\sigma^2_{xy}/(\sigma_x\sigma_y))$
\pagebreak

$\sum_i -\ln(v_i)v_i$
\pagebreak

$\ln(2)$
\pagebreak

$\int -\ln(p(x))p(x)dx$
\pagebreak

$-\ln(p(x))$
\pagebreak

$ D(p,q) = \sum_i \ln(p_i/q_i) p_i $
\pagebreak

$q$
\pagebreak

$D(p, q) \neq D(q, p)$
\pagebreak

$p_i>0$
\pagebreak

$q_i=0$
\pagebreak

\[ \Gamma_p(a)= \pi^{p(p-1)/4}\prod_{j=1}^p \Gamma\left[ a+(1-j)/2\right]. \]
\pagebreak

$\Gamma(x)$
\pagebreak

$x\in\{0, -1, -2, ...\}$
\pagebreak

$a+(1-j)/2$
\pagebreak

$L > R$
\pagebreak

\[{N-K\over q} {({\bf Q}'\hat\beta - {\bf c})' [{\bf Q}' ({\bf X}'{\bf X})^{-1} {\bf Q}]^{-1} ({\bf Q}' \hat\beta - {\bf c}) \over {\bf u}' {\bf u} } \sim F_{q,N-K},\]
\pagebreak

${\bf Q}$
\pagebreak

${\bf c}$
\pagebreak

$\beta_1$
\pagebreak

$(X'X)^{-1}$
\pagebreak

$(X'\Sigma X)^{-1}$
\pagebreak

$F$
\pagebreak

$\lambda^{-1}$
\pagebreak

$\lambda$
\pagebreak

$\rightarrow$
\pagebreak

$0, 1, 2, ...$
\pagebreak

$[0, 1]$
\pagebreak

$(n-1)/n$
\pagebreak

$(n-1)(n-2)/n^2$
\pagebreak

$\sqrt{x}$
\pagebreak

$x^y$
\pagebreak

$e^x$
\pagebreak

$\ln(x)$
\pagebreak

$\sin(x)$
\pagebreak

$\arcsin(x)$
\pagebreak

$\lambda=2.8$
\pagebreak

$2.0$
\pagebreak

$1.3$
\pagebreak

$(\lambda)$
\pagebreak

$x>0$
\pagebreak

$(d_1)$
\pagebreak

$(\mu, \sigma)$
\pagebreak

$d_2$
\pagebreak

$(d_1, d_2)$
\pagebreak

$(\mu, \sigma, \lambda)$
\pagebreak

$\beta_0$
\pagebreak

$X\beta$
\pagebreak

${\partial\over \partial\beta}\log L(\beta)'I^{-1}(\beta){\partial\over \partial\beta}\log L(\beta)$
\pagebreak

$L$
\pagebreak

$I$
\pagebreak

$\sim \chi^2_m$
\pagebreak

$m$
\pagebreak

$(1-x)^2+ s(y - x^2)^2$
\pagebreak

$s$
\pagebreak

$(i,j)$
\pagebreak

$AIC_c$
\pagebreak

$BIC$
\pagebreak

$y = x_1 + \log(x_2) + x_3^2$
\pagebreak

$x_1$
\pagebreak

$n/K$
\pagebreak

$<$
\pagebreak

$\geq 0$
\pagebreak

$X'\beta$
\pagebreak

$n=30$
\pagebreak

$p_1$
\pagebreak

$Z(a) = {1\over \zeta(a) * i^a} $
\pagebreak

$lnZ(a) = -(\log(\zeta(a)) + a \log(i)) $
\pagebreak

$P(x) = 1$
\pagebreak

$ Y(x, b) = (b-1) \gamma(b) \gamma(k) / \gamma(k+b) $
\pagebreak

$ \ln Y(x, b) = \ln(b-1) + ln\gamma(b) + \ln\gamma(k) - \ln\gamma(k+b) $
\pagebreak

$ d\ln Y/db = 1/(b-1) + \psi(b) - \psi(k+b) $
\pagebreak

$j$
\pagebreak

$e^{x\beta_j}/ (\sum_i{e^{x\beta_i}})$
\pagebreak

$x\beta_j - ln(\sum_i{e^{x\beta_i}})$
\pagebreak

$f = exp(-(ln(x)-\mu)^2/(2\sigma^2))/ (x\sigma\sqrt{2\pi})$
\pagebreak

$ln f = -(ln(x)-\mu)^2/(2\sigma^2) - ln(x) - ln(\sigma\sqrt{2\pi})$
\pagebreak

$df$
\pagebreak

$P(d)$
\pagebreak

$d$
\pagebreak

$G(x, a, b) = {1\over (\Gamma(a) b^a)} x^{a-1} e^{-x/b}$
\pagebreak

$ln G(x, a, b)= -ln \Gamma(a) - a ln b + (a-1)ln(x) + -x/b$
\pagebreak

$d ln G/ da = -\psi(a) - ln b + ln(x) $
\pagebreak

$d ln \gamma = \psi$
\pagebreak

$d ln G/ db = -a/b + x/(b^2) $
\pagebreak

$p(k) = {\mu^k \over k!} \exp(-\mu). $
\pagebreak

$N(\mu,\sigma^2) = {1 \over \sqrt{2 \pi \sigma^2}} \exp (-x^2 / 2\sigma^2)$
\pagebreak

$\ln N(\mu,\sigma^2) = (-(x-\mu)^2 / 2\sigma^2) - \ln (2 \pi \sigma^2)/2 $
\pagebreak

$d\ln N(\mu,\sigma^2)/d\mu = (x-\mu) / \sigma^2 $
\pagebreak

$d\ln N(\mu,\sigma^2)/d\sigma^2 = ((x-\mu)^2 / 2(\sigma^2)^2) - 1/2\sigma^2 $
\pagebreak

$Z(\mu,k) = \sum_k 1/\mu e^{-k/\mu} $
\pagebreak

$ln Z(\mu,k) = \sum_k -\ln(\mu) - k/\mu $
\pagebreak

$dln Z(\mu,k)/d\mu = \sum_k -1/\mu + k/(\mu^2) $
\pagebreak

$Z(C,k) = \ln C C^{-k}. $
\pagebreak

$\mu = {1\over \ln C}$
\pagebreak

$C=\exp(1/\mu)$
\pagebreak

$p_0$
\pagebreak

$p_0=1-\sum_{i=1}^{k-1} p_i$
\pagebreak

$k \times k$
\pagebreak

$1\times 1$
\pagebreak

$ Y = \beta X + \epsilon$
\pagebreak

$\beta X$
\pagebreak

$P(Y|X\beta) \sim {\cal N}(X\beta, \sigma)$
\pagebreak

$P(X)=1$
\pagebreak

$P(Y, X) = P(Y|X)P(X) = P(Y|X)$
\pagebreak

$X\beta+\epsilon$
\pagebreak

$\times$
\pagebreak

$\in[0,1]$
\pagebreak

$v[1]>1$
\pagebreak

$a$
\pagebreak

$b$
\pagebreak

$p(1-p)$
\pagebreak

\end{document}
